Launchbury/CoCallAnalysisBinds.thy
@@ -1,5 +1,5 @@
 theory CoCallAnalysisBinds
-imports CoCallAnalysis AEnv
+imports CoCallAnalysis AEnv  "AList-Utils-HOLCF"
 begin
 
 context CoCallAnalysis
@@ -24,33 +24,68 @@ lemma ccBind_eq[simp]: "ccBind v e \<cdot> (ae, G) = (if (v--v\<notin>G) \<or> \
 lemma ccBind_strict[simp]: "ccBind v e \<cdot> \<bottom> = \<bottom>"
   by (auto simp add: inst_prod_pcpo simp del: Pair_strict)
 
+(*
 fun ccBinds :: "heap \<Rightarrow> ((AEnv \<times> CoCalls) \<rightarrow> CoCalls)"
   where "ccBinds [] = csnd"
      |  "ccBinds ((v,e)#binds) = ccBind v e \<squnion> ccBinds (delete v binds)"
+*)
+term lub
+definition ccBinds :: "heap \<Rightarrow> ((AEnv \<times> CoCalls) \<rightarrow> CoCalls)"
+  where "ccBinds \<Gamma> = (\<Lambda> i. (\<Squnion>v\<mapsto>e\<in>map_of \<Gamma>. ccBind v e\<cdot>i))"
+lemma ccBinds_eq:
+  "ccBinds \<Gamma>\<cdot>i = (\<Squnion>v\<mapsto>e\<in>map_of \<Gamma>. ccBind v e\<cdot>i)" sorry
 
 lemma ccBinds_strict[simp]: "ccBinds \<Gamma>\<cdot>\<bottom>=\<bottom>"
-  by (induct \<Gamma> rule: ccBinds.induct) auto
+  unfolding ccBinds_eq
+  by (cases "\<Gamma> = []") simp_all
 
 lemma ccBinds_strict'[simp]: "ccBinds \<Gamma>\<cdot>(\<bottom>,\<bottom>)=\<bottom>"
-  by (induct \<Gamma> rule: ccBinds.induct) auto
+  by (metis CoCallAnalysis.ccBinds_strict Pair_bottom_iff)
 
-lemma ccBinds_reorder1: "map_of \<Gamma> v = Some e \<Longrightarrow> ccBinds \<Gamma> = ccBind v e \<squnion> ccBinds (delete v \<Gamma>)"
-proof (induction \<Gamma> rule: ccBinds.induct)
-  case 1 thus ?case by simp
-next
-  case (2 v' e' \<Gamma>)
-  thus ?case
-  by (cases "v' = v") (auto simp add: delete_twist)
+lemma ccBinds_fun_upd[simp]:
+  "(\<Squnion>k\<mapsto>v\<in>m(k' \<mapsto> v'). e k v) = e k' v' \<squnion> (\<Squnion>k\<mapsto>v\<in>m(k':=None). e k v)"
+ sorry
+
+lemma ccBinds_reorder1:
+  assumes "map_of \<Gamma> v = Some e"
+  shows "ccBinds \<Gamma> = ccBind v e \<squnion> ccBinds (delete v \<Gamma>)"
+proof-
+  from assms 
+  have "map_of \<Gamma> = map_of ((v,e) # delete v \<Gamma>)" by (metis map_of_delete_insert)
+  thus ?thesis
+    by (auto intro: cfun_eqI simp add: ccBinds_eq delete_set_none)
 qed
 
-definition ccBindsExtra :: "heap \<Rightarrow> ((AEnv \<times> CoCalls) \<rightarrow> CoCalls)"
-  where "ccBindsExtra \<Gamma> = (\<Lambda> i.  ccBinds \<Gamma> \<cdot> i \<squnion> ccProd (fv \<Gamma> - domA \<Gamma>) (ccNeighbors (domA \<Gamma>) (ccBinds \<Gamma> \<cdot> i)))"
+lemma ccBind_below_ccBinds: "map_of \<Gamma> x = Some e \<Longrightarrow> ccBind x e\<cdot>ae \<sqsubseteq> (ccBinds \<Gamma>\<cdot>ae)"
+  by (auto simp add: ccBinds_eq)
 
-lemma ccBindsExtra_simp: "ccBindsExtra \<Gamma> \<cdot> i = ccBinds \<Gamma> \<cdot> i \<squnion> ccProd (fv \<Gamma> - domA \<Gamma>) (ccNeighbors (domA \<Gamma>) (ccBinds \<Gamma> \<cdot> i))"
+(*
+lemma ccBinds_lub: "ccBinds \<Gamma>\<cdot>(ae,G) = lub {ccBind x e\<cdot>(ae,G) | x e . map_of \<Gamma> x = Some e} \<squnion> G"
+proof (induction rule: ccBinds.induct[case_names Nil Cons])
+  case Nil thus ?case by simp
+next
+  case (Cons v e \<Gamma>)
+  have "{ccBind x ea\<cdot>(ae, G) |x ea. map_of ((v, e) # \<Gamma>) x = Some ea} =
+        insert (ccBind v e\<cdot>(ae, G)) {ccBind x ea\<cdot>(ae, G) |x ea. map_of (delete v \<Gamma>) x = Some ea}"
+    by auto
+  hence "lub {ccBind x ea\<cdot>(ae, G) |x ea. map_of ((v, e) # \<Gamma>) x = Some ea}
+     = ccBind v e\<cdot>(ae, G) \<squnion> lub {ccBind x ea\<cdot>(ae, G) |x ea. map_of (delete v \<Gamma>) x = Some ea}"
+     by (simp only: lub_insert)
+  thus ?case
+    using Cons by simp
+qed
+*)     
+
+definition ccBindsExtra :: "heap \<Rightarrow> ((AEnv \<times> CoCalls) \<rightarrow> CoCalls)"
+  where "ccBindsExtra \<Gamma> = (\<Lambda> i.  snd i \<squnion> ccBinds \<Gamma> \<cdot> i  \<squnion> (\<Squnion>x\<mapsto>e\<in>map_of \<Gamma>. ccProd (fv e) (ccNeighbors (domA \<Gamma>) (snd i))))"
+
+
+lemma ccBindsExtra_simp: "ccBindsExtra \<Gamma> \<cdot> i = snd i \<squnion> ccBinds \<Gamma> \<cdot> i \<squnion> (\<Squnion>x\<mapsto>e\<in>map_of \<Gamma>. ccProd (fv e) (ccNeighbors (domA \<Gamma>) (snd i)))"
   unfolding ccBindsExtra_def by simp
 
 lemma ccBindsExtra_strict[simp]: "ccBindsExtra \<Gamma> \<cdot> \<bottom> = \<bottom>"
   by (auto simp add: ccBindsExtra_simp inst_prod_pcpo simp del: Pair_strict)
+
 end
 
 lemma ccBind_eqvt[eqvt]: "\<pi> \<bullet> (CoCallAnalysis.ccBind cccExp x e) = CoCallAnalysis.ccBind (\<pi> \<bullet> cccExp) (\<pi> \<bullet> x) (\<pi> \<bullet> e)"
@@ -66,9 +101,9 @@ qed
 
 lemma ccBinds_eqvt[eqvt]: "\<pi> \<bullet> (CoCallAnalysis.ccBinds cccExp \<Gamma>) = CoCallAnalysis.ccBinds (\<pi> \<bullet> cccExp) (\<pi> \<bullet> \<Gamma>)"
   apply (rule cfun_eqvtI)
-  apply (induction \<Gamma> rule: CoCallAnalysis.ccBinds.induct)
-  apply (simp add: CoCallAnalysis.ccBinds.simps)
-  apply (simp add: CoCallAnalysis.ccBinds.simps, perm_simp, simp)
+  unfolding CoCallAnalysis.ccBinds_eq
+  apply (perm_simp) 
+  apply rule
   done
 
 lemma ccBindsExtra_eqvt[eqvt]: "\<pi> \<bullet> (CoCallAnalysis.ccBindsExtra cccExp \<Gamma>) = CoCallAnalysis.ccBindsExtra (\<pi> \<bullet> cccExp) (\<pi> \<bullet> \<Gamma>)"
@@ -88,18 +123,25 @@ lemma ccBind_cong[fundef_cong]:
 lemma ccBinds_cong[fundef_cong]:
   "\<lbrakk> (\<And> e. e \<in> snd ` set heap2 \<Longrightarrow> cccexp1 e = cccexp2 e); heap1 = heap2 \<rbrakk>
       \<Longrightarrow> CoCallAnalysis.ccBinds cccexp1 heap1 = CoCallAnalysis.ccBinds cccexp2 heap2"
-  apply simp
-  apply (induction heap2 arbitrary: heap1 rule: CoCallAnalysis.ccBinds.induct)
-  apply (simp add: CoCallAnalysis.ccBinds.simps)
-  apply (simp add: CoCallAnalysis.ccBinds.simps)
-  by (metis "AList-Utils.dom_delete_subset" ccBind_cong contra_subsetD)
- 
+  apply (rule cfun_eqI)
+  unfolding CoCallAnalysis.ccBinds_eq
+  apply (rule arg_cong[OF mapCollect_cong])
+  apply (rule arg_cong[OF ccBind_cong])
+  apply auto
+  by (metis imageI map_of_is_SomeD snd_conv)
+
 lemma ccBindsExtra_cong[fundef_cong]:
   "\<lbrakk> (\<And> e. e \<in> snd ` set heap2 \<Longrightarrow> cccexp1 e = cccexp2 e); heap1 = heap2 \<rbrakk>
       \<Longrightarrow> CoCallAnalysis.ccBindsExtra cccexp1 heap1 = CoCallAnalysis.ccBindsExtra cccexp2 heap2"
-  unfolding CoCallAnalysis.ccBindsExtra_def
-  by (metis (mono_tags, hide_lams) ccBinds_cong)
-
+  apply (rule cfun_eqI)
+  unfolding CoCallAnalysis.ccBindsExtra_simp
+  apply (rule arg_cong2[OF ccBinds_cong mapCollect_cong]) 
+  apply simp+
+  (*
+  apply (rule arg_cong[OF ccBinds_cong])
+  apply simp+
+  *)
+  done
 
 
 end
