Launchbury/CoCallAnalysis.thy
@@ -23,6 +23,8 @@ locale CoCallAnalysis_ccField = CoCallAnalysis +
   assumes "ccField (ccExp e\<cdot>a) \<subseteq> fv e"
 
 locale CoCallAnalyisHeap = 
+  fixes calledOnce :: "heap \<Rightarrow> exp \<Rightarrow> Arity \<Rightarrow> var set"
+  fixes isLinear :: "heap \<Rightarrow> exp \<Rightarrow> Arity \<Rightarrow> bool"
   fixes ccHeap :: "heap \<Rightarrow> exp \<Rightarrow> Arity \<rightarrow> CoCalls"
 
 
